changing environment

src/Executable_Facts.v
@@ -1,4 +1,4 @@
-Require Import Term_Defs_Core Manifest Manifest_Generator Manifest_Generator_Facts Executable_Defs_Prop.
+Require Import Term_Defs_Core Manifest Manifest_Generator Manifest_Generator_Facts Executable_Defs_Prop Manifest_Admits.
 
 Require Import List.
 Import ListNotations.
@@ -22,30 +22,45 @@ Definition Environment := Plc -> option Manifest.
 Print Manifest. 
 Print Environment.
 
-Definition canRunAsp_Env (k:Plc) (e:Environment) (a: ASP_ID) : Prop := 
-  match (e k) with 
-  | None => False
-  | Some m => In a m.(asps)
-  end.
+Definition canRunAsp_Env (k:Plc) (em:EnvironmentM) (a: ASP_ID) : Prop := 
+  match (Maps.map_get em k) with 
+  | None => False 
+  | Some m => In k m.(asps)
+  end. 
+  
   
 Print EnvironmentM.
 (*  Maps.MapC Plc Manifest *)
+
 Print knowsOf_Manifest.
 
-Definition knowsOf_Env (k:Plc)(e:Environment)(p:Plc):Prop :=
-  match (e k) with
+Definition knowsOf_Env (k:Plc)(em:EnvironmentM)(p:Plc):Prop :=
+  match (Maps.map_get em k) with 
   | None => False
   | Some m => In p m.(uuidPlcs)
   end.
 
-Fixpoint executable_static (t:Term) (k:Plc) (e:Environment) : Prop := 
+(* Statically, we have a global view so we can use the environement to reason about the system *)
+Fixpoint executable_static (t:Term) (k:Plc) (em:EnvironmentM) : Prop := 
   match t with
-    | asp (ASPC _ _ (asp_paramsC asp_id _ _ _))  => canRunAsp_Env k e asp_id
+    | asp (ASPC _ _ (asp_paramsC asp_id _ _ _))  => canRunAsp_Env k em asp_id
     | asp _ => True
-    | att p t => knowsOf_Env k e p -> executable_static t k e
-    | lseq t1 t2 => executable_static t1 k e /\ executable_static t2 k e
-    | bseq _ t1 t2 => executable_static t1 k e /\ executable_static t2 k e
-    | bpar _ t1 t2 => executable_static t1 k e /\ executable_static t2 k e
+    | att p t => knowsOf_Env k em p -> executable_static t k em
+    | lseq t1 t2 => executable_static t1 k em /\ executable_static t2 k em
+    | bseq _ t1 t2 => executable_static t1 k em /\ executable_static t2 k em
+    | bpar _ t1 t2 => executable_static t1 k em /\ executable_static t2 k em
+  end.
+
+(* A dynamic version of executabiilty. 
+   At runtime, we cannot know if an att term can be executed on a remote place. *)
+Fixpoint executable_dynamic (t:Term) (k:Plc) (em:EnvironmentM) : Prop := 
+  match t with
+    | asp (ASPC _ _ (asp_paramsC asp_id _ _ _))  => canRunAsp_Env k em asp_id
+    | asp _ => True
+    | att p t => knowsOf_Env k em p
+    | lseq t1 t2 => executable_dynamic t1 k em /\ executable_dynamic t2 k em
+    | bseq _ t1 t2 => executable_dynamic t1 k em /\ executable_dynamic t2 k em
+    | bpar _ t1 t2 => executable_dynamic t1 k em /\ executable_dynamic t2 k em
   end.
 
 Definition envs_eq_at (e:Environment) (em:EnvironmentM) (ps:list Plc) : Prop := 
@@ -53,12 +68,49 @@ Definition envs_eq_at (e:Environment) (em:EnvironmentM) (ps:list Plc) : Prop :=
         In p ps ->
         e p = Maps.map_get em p.
 
+(* Record Manifest : Set := Build_Manifest
+                            { my_abstract_plc : Plc;
+                              asps : list ASP_ID;
+                              uuidPlcs : list Plc;
+                              pubKeyPlcs : list Plc;
+                              policy : Manifest_Admits.PolicyT }.*)
+
+(* Try to build a manifest. *)
+
+Definition build_manifest_helper p a p1 p2 pol : Manifest := 
+{|  my_abstract_plc := p ; 
+    asps :=  a ;
+    uuidPlcs := p1 ; 
+    pubKeyPlcs := p2 ; 
+    policy := pol |}. 
 
 (* Proof that the dynamic notion of executability respects the static notion of executability. *)
 Theorem static_executability_implies_distributed : 
-    forall t p e em,
-      envs_eq_at e em (places p t) ->
-      executable_static t p e -> 
+    forall t p em,
+      executable_static t p em -> 
       distributed_executability t p em.
 Proof.
+  intros. unfold distributed_executability. intros; subst.
+  induction t.  
+  + destruct a eqn:H'.
+  ++ induction em.
+  +++ simpl in *; auto. split with (x := (build_manifest_helper p0 [] [] [] empty_PolicyT) ).
+  +++ left.    
+  remember (build_manifest_helper p0 [] [] [] empty_PolicyT) as m.
+
+  
+  
+  inversion H1; simpl in *. 
+  
+  
+  
+  
+  
+  
+  inversion H.   remember (build_manifest_helper p0 [] [] [] empty_PolicyT) as m.
+     exists m. split.
+  +++ simpl in *.      
+  
+  destruct em eqn:H'.
+  ++ split with (x := []).  split with (x := a).
 Abort.
